Add worlds to ThreadQueue, unfortunately drawing in Axiom K

platform/ThreadQueue.v
@@ -4,8 +4,21 @@ Import W_W_Bag.
 Set Implicit Arguments.
 
 
+Record tq_args (world : Type) := {
+  World : world;
+  Pointer : W;
+  Settings : settings;
+  Mem : smem
+}.
+
 Module Type S.
-  Variable globalInv : W -> hpropB ((settings * state : Type)%type :: nil).
+  Variable world : Type.
+
+  Variable evolve : world -> world -> Prop.
+  Axiom evolve_refl : forall w, evolve w w.
+  Axiom evolve_trans : forall w1 w2 w3, evolve w1 w2 -> evolve w2 w3 -> evolve w1 w3.
+
+  Variable globalInv : world -> W -> hpropB (tq_args world :: nil).
 End S.
 
 Module Make(M : S).
@@ -13,35 +26,51 @@ Import M.
 
 (* What does it mean for a program counter to be valid for a suspended thread? *)
 
-Definition susp (sc pc sp : W) : HProp := fun s m =>
+Definition susp (w : world) (sc pc sp : W) : HProp := fun s m =>
   (Ex pc_tq : W, [| s.(Labels) ("threadq"!"ADT")%SP = Some pc_tq |]
-    /\ ExX (* tq *) : settings * state, Cptr pc_tq #0
+    /\ ExX (* tq *) : tq_args world, Cptr pc_tq (_ ~> PropX.Forall #0)
     /\ ExX (* pre *) : settings * state, Cptr pc #0
     /\ ExX (* inv *) : settings * smem, #0 (s, m)
-    /\ Al st : settings * state,
-    ![ #0 * ##2 sc * (fun x y => Lift (Lift (globalInv sc x y))) * ^[mallocHeap 0] ] st
+    /\ Al st : settings * state, Al w' : world,
+    [| evolve w w' |]
+    /\ ![ #0 * (fun x y => Lift (Lift (Var0 {| World := w';
+                                               Pointer := sc;
+                                               Settings := x;
+                                               Mem := y |})))
+      * (fun x y => Lift (Lift (globalInv w' sc x y)))
+      * ^[mallocHeap 0] ] st
     /\ [| st#Sp = sp |]
     ---> #1 st)%PropX.
 
-Lemma susp_intro : forall specs sc pc sp P stn st,
+Lemma susp_intro : forall specs w sc pc sp P stn st,
   (exists pc_tq, stn.(Labels) ("threadq"!"ADT")%SP = Some pc_tq
-    /\ exists tq, specs pc_tq = Some (fun x => tq x)
+    /\ exists tq, specs pc_tq = Some (fun _ => PropX.Forall tq)
       /\ exists pre, specs pc = Some (fun x => pre x)
         /\ exists inv, interp specs (![ inv * P ] (stn, st))
-          /\ forall stn_st, interp specs (![ inv * predIn tq sc * substH (globalInv sc) tq * mallocHeap 0 ] stn_st
+          /\ forall stn_st w', interp specs ([| evolve w w' |]
+            /\ ![ inv
+              * (fun x y => tq {| World := w';
+                                  Pointer := sc;
+                                  Settings := x;
+                                  Mem := y |})
+              * substH (globalInv w' sc) tq * mallocHeap 0 ] stn_st
             /\ [| stn_st#Sp = sp |]
             ---> pre stn_st)%PropX)
-  -> interp specs (![ susp sc pc sp * P ] (stn, st)).
+  -> interp specs (![ susp w sc pc sp * P ] (stn, st)).
   cptr.
 Qed.
 
-Lemma susp_elim : forall specs sc pc sp P stn st,
-  interp specs (![ susp sc pc sp * P ] (stn, st))
+Lemma susp_elim : forall specs w sc pc sp P stn st,
+  interp specs (![ susp w sc pc sp * P ] (stn, st))
   -> (exists pc_tq, stn.(Labels) ("threadq"!"ADT")%SP = Some pc_tq
-    /\ exists tq, specs pc_tq = Some (fun x => tq x)
+    /\ exists tq, specs pc_tq = Some (fun _ => PropX.Forall tq)
       /\ exists pre, specs pc = Some (fun x => pre x)
         /\ exists inv, interp specs (![ inv * P ] (stn, st))
-          /\ forall stn_st, interp specs (![ inv * predIn tq sc * substH (globalInv sc) tq * mallocHeap 0 ] stn_st
+          /\ forall stn_st w', interp specs ([| evolve w w' |]
+            /\ ![ inv * (fun x y => tq {| World := w';
+                                          Pointer := sc;
+                                          Settings := x;
+                                          Mem := y |}) * substH (globalInv w' sc) tq * mallocHeap 0 ] stn_st
             /\ [| stn_st#Sp = sp |]
             ---> pre stn_st)%PropX).
   cptr.
@@ -49,6 +78,7 @@ Lemma susp_elim : forall specs sc pc sp P stn st,
   descend; eauto.
   rewrite <- sepFormula_eq; descend.
   step auto_ext.
+  eauto.
   make_Himp.
   apply Himp_refl.
 Qed.
@@ -60,65 +90,65 @@ Inductive splitSusp : Prop := SS.
 Hint Constructors mergeSusp splitSusp.
 
 Module Type TQ.
-  Parameter susps : bag -> W -> HProp.
-  Parameter tq : W -> HProp.
+  Parameter susps : world -> bag -> W -> HProp.
+  Parameter tq : world -> W -> HProp.
 
-  Axiom tq_extensional : forall sc, HProp_extensional (tq sc).
+  Axiom tq_extensional : forall w sc, HProp_extensional (tq w sc).
 
-  Axiom susps_empty_bwd : forall sc, Emp ===> susps empty sc.
-  Axiom susps_add_bwd : forall sc b pc sp, pc = pc -> mergeSusp -> susp sc pc sp * susps b sc ===> susps (b %+ (pc, sp)) sc.
-  Axiom susps_del_fwd : forall sc b pc sp, (pc, sp) %in b -> susps b sc ===> susp sc pc sp * susps (b %- (pc, sp)) sc.
+  Axiom susps_empty_bwd : forall w sc, Emp ===> susps w empty sc.
+  Axiom susps_add_bwd : forall w sc b pc sp, pc = pc -> mergeSusp -> susp w sc pc sp * susps w b sc ===> susps w (b %+ (pc, sp)) sc.
+  Axiom susps_del_fwd : forall w sc b pc sp, (pc, sp) %in b -> susps w b sc ===> susp w sc pc sp * susps w (b %- (pc, sp)) sc.
 
   (* Below, the extra [locals] is a temporary stack for the threadq to use during sensitive
    * stack manipulations when the threads' own stacks may not be safe to touch. *)
 
-  Axiom tq_fwd : forall sc, tq sc ===> Ex b, Ex p, Ex sp, Ex vs, (sc ==*> p, sp) * (sc ^+ $8) =?> 2
+  Axiom tq_fwd : forall w sc, tq w sc ===> Ex b, Ex p, Ex sp, Ex vs, (sc ==*> p, sp) * (sc ^+ $8) =?> 2
     * locals ("rp" :: "sc" :: "q" :: "curPc" :: "curSp" :: "newPc" :: "newSp" :: nil) vs 14 sp
-    * queue b p * susps b sc * any.
+    * queue b p * susps w b sc * any.
 
-  Axiom tq_bwd : forall sc, (Ex b, Ex p, Ex sp, Ex vs, (sc ==*> p, sp) * (sc ^+ $8) =?> 2
+  Axiom tq_bwd : forall w sc, (Ex b, Ex p, Ex sp, Ex vs, (sc ==*> p, sp) * (sc ^+ $8) =?> 2
     * locals ("rp" :: "sc" :: "q" :: "curPc" :: "curSp" :: "newPc" :: "newSp" :: nil) vs 14 sp
-    * queue b p * susps b sc * any) ===> tq sc.
+    * queue b p * susps w b sc * any) ===> tq w sc.
 End TQ.
 
 Module Tq : TQ.
   Open Scope Sep_scope.
 
-  Definition susps (b : bag) (sc : W) : HProp :=
-    starB (fun p => susp sc (fst p) (snd p)) b.
+  Definition susps (w : world) (b : bag) (sc : W) : HProp :=
+    starB (fun p => susp w sc (fst p) (snd p)) b.
 
-  Theorem susps_empty_bwd : forall sc, Emp ===> susps empty sc.
+  Theorem susps_empty_bwd : forall w sc, Emp ===> susps w empty sc.
     intros; apply starB_empty_bwd.
   Qed.
 
-  Theorem susps_add_bwd : forall sc b pc sp, pc = pc -> mergeSusp -> susp sc pc sp * susps b sc ===> susps (b %+ (pc, sp)) sc.
+  Theorem susps_add_bwd : forall w sc b pc sp, pc = pc -> mergeSusp -> susp w sc pc sp * susps w b sc ===> susps w (b %+ (pc, sp)) sc.
     intros; eapply Himp_trans; [ | apply starB_add_bwd ].
     unfold susps; simpl.
     apply Himp_star_comm.
   Qed.
 
-  Theorem susps_del_fwd : forall sc b pc sp, (pc, sp) %in b -> susps b sc ===> susp sc pc sp * susps (b %- (pc, sp)) sc.
+  Theorem susps_del_fwd : forall w sc b pc sp, (pc, sp) %in b -> susps w b sc ===> susp w sc pc sp * susps w (b %- (pc, sp)) sc.
     intros; eapply Himp_trans; [ apply starB_del_fwd; eauto | apply Himp_refl ].
   Qed.
 
-  Definition tq (sc : W) : HProp :=
+  Definition tq (w : world) (sc : W) : HProp :=
     Ex b, Ex p, Ex sp, Ex vs, (sc ==*> p, sp) * (sc ^+ $8) =?> 2
       * locals ("rp" :: "sc" :: "q" :: "curPc" :: "curSp" :: "newPc" :: "newSp" :: nil) vs 14 sp
-      * queue b p * susps b sc * any.
+      * queue b p * susps w b sc * any.
 
-  Theorem tq_extensional : forall sc, HProp_extensional (tq sc).
+  Theorem tq_extensional : forall w sc, HProp_extensional (tq w sc).
     reflexivity.
   Qed.
 
-  Theorem tq_fwd : forall sc, tq sc ===> Ex b, Ex p, Ex sp, Ex vs, (sc ==*> p, sp) * (sc ^+ $8) =?> 2
+  Theorem tq_fwd : forall w sc, tq w sc ===> Ex b, Ex p, Ex sp, Ex vs, (sc ==*> p, sp) * (sc ^+ $8) =?> 2
     * locals ("rp" :: "sc" :: "q" :: "curPc" :: "curSp" :: "newPc" :: "newSp" :: nil) vs 14 sp
-    * queue b p * susps b sc * any.
+    * queue b p * susps w b sc * any.
     unfold tq; sepLemma.
   Qed.
 
-  Theorem tq_bwd : forall sc, (Ex b, Ex p, Ex sp, Ex vs, (sc ==*> p, sp) * (sc ^+ $8) =?> 2
+  Theorem tq_bwd : forall w sc, (Ex b, Ex p, Ex sp, Ex vs, (sc ==*> p, sp) * (sc ^+ $8) =?> 2
     * locals ("rp" :: "sc" :: "q" :: "curPc" :: "curSp" :: "newPc" :: "newSp" :: nil) vs 14 sp
-    * queue b p * susps b sc * any) ===> tq sc.
+    * queue b p * susps w b sc * any) ===> tq w sc.
     unfold tq; sepLemma.
   Qed.
 End Tq.
@@ -133,40 +163,44 @@ Defined.
 
 (* What is a valid initial code pointer for a thread, given the requested stack size? *)
 
-Definition ginv sc := substH (globalInv sc) (predOut tq).
+Definition ginv w sc := substH (globalInv w sc) (fun x => tq (World x) (Pointer x) (Settings x) (Mem x)).
 
-Definition starting (sc pc : W) (ss : nat) : HProp := fun s m =>
+Definition starting (w : world) (sc pc : W) (ss : nat) : HProp := fun s m =>
   (ExX (* pre *) : settings * state, Cptr pc #0
     /\ [| semp m |]
-    /\ Al st : settings * state, Al vs,
-      ![ ^[locals ("rp" :: "sc" :: nil) vs ss st#Sp * tq sc * ginv sc * mallocHeap 0] ] st
+    /\ Al st : settings * state, Al vs, Al w',
+      [| evolve w w' |]
+      /\ ![ ^[locals ("rp" :: "sc" :: nil) vs ss st#Sp * tq w' sc * ginv w' sc * mallocHeap 0] ] st
       /\ [| sel vs "sc" = sc |]
       ---> #0 st)%PropX.
 
 Local Hint Resolve split_a_semp_a semp_smem_emp.
 
-Lemma starting_intro : forall specs sc pc ss P stn st,
+Lemma starting_intro : forall specs sc w pc ss P stn st,
   (exists pre, specs pc = Some (fun x => pre x)
     /\ interp specs (![ P ] (stn, st))
-    /\ forall stn_st vs, interp specs (![ locals ("rp" :: "sc" :: nil) vs ss stn_st#Sp
-      * tq sc * ginv sc * mallocHeap 0 ] stn_st
+    /\ forall stn_st vs w', interp specs ([| evolve w w' |]
+      /\ ![ locals ("rp" :: "sc" :: nil) vs ss stn_st#Sp
+      * tq w' sc * ginv w' sc * mallocHeap 0 ] stn_st
     /\ [| sel vs "sc" = sc |]
     ---> pre stn_st)%PropX)
-  -> interp specs (![ starting sc pc ss * P ] (stn, st)).
+  -> interp specs (![ starting w sc pc ss * P ] (stn, st)).
   cptr.
 Qed.
 
-Lemma starting_elim : forall specs sc pc ss P stn st,
-  interp specs (![ starting sc pc ss * P ] (stn, st))
+Lemma starting_elim : forall specs w sc pc ss P stn st,
+  interp specs (![ starting w sc pc ss * P ] (stn, st))
   -> (exists pre, specs pc = Some (fun x => pre x)
     /\ interp specs (![ P ] (stn, st))
-    /\ forall stn_st vs, interp specs (![ locals ("rp" :: "sc" :: nil) vs ss stn_st#Sp
-      * tq sc * ginv sc * mallocHeap 0 ] stn_st
+    /\ forall stn_st vs w', interp specs ([| evolve w w' |]
+      /\ ![ locals ("rp" :: "sc" :: nil) vs ss stn_st#Sp
+      * tq w' sc * ginv w' sc * mallocHeap 0 ] stn_st
     /\ [| sel vs "sc" = sc |]
     ---> pre stn_st)%PropX).
   cptr.
   generalize (split_semp _ _ _ H0 H); intros; subst; auto.
   rewrite <- sepFormula_eq; descend; step auto_ext.
+  eauto.
   make_Himp.
   apply Himp_refl.
   assumption.
@@ -174,23 +208,28 @@ Qed.
 
 
 Definition initS : spec := SPEC reserving 12
+  Al w,
   PRE[_] mallocHeap 0
-  POST[R] tq R * mallocHeap 0.
+  POST[R] tq w R * mallocHeap 0.
 
 Definition spawnWithStackS : spec := SPEC("sc", "pc", "sp") reserving 14
-  PRE[V] tq (V "sc") * susp (V "sc") (V "pc") (V "sp") * mallocHeap 0
-  POST[_] tq (V "sc") * mallocHeap 0.
+  Al w,
+  PRE[V] tq w (V "sc") * susp w (V "sc") (V "pc") (V "sp") * mallocHeap 0
+  POST[_] tq w (V "sc") * mallocHeap 0.
 
 Definition spawnS : spec := SPEC("sc", "pc", "ss") reserving 18
-  PRE[V] [| V "ss" >= $2 |] * tq (V "sc") * starting (V "sc") (V "pc") (wordToNat (V "ss") - 2) * mallocHeap 0
-  POST[_] tq (V "sc") * mallocHeap 0.
+  Al w,
+  PRE[V] [| V "ss" >= $2 |] * tq w (V "sc") * starting w (V "sc") (V "pc") (wordToNat (V "ss") - 2) * mallocHeap 0
+  POST[_] tq w (V "sc") * mallocHeap 0.
 
 Definition exitS : spec := SPEC("sc") reserving 12
-  PREonly[V] tq (V "sc") * ginv (V "sc") * mallocHeap 0.
+  Al w,
+  PREonly[V] tq w (V "sc") * ginv w (V "sc") * mallocHeap 0.
 
 Definition yieldS : spec := SPEC("sc") reserving 19
-  PRE[V] tq (V "sc") * ginv (V "sc") * mallocHeap 0
-  POST[_] tq (V "sc") * ginv (V "sc") * mallocHeap 0.
+  Al w,
+  PRE[V] tq w (V "sc") * ginv w (V "sc") * mallocHeap 0
+  POST[_] Ex w', [| evolve w w' |] * tq w' (V "sc") * ginv w' (V "sc") * mallocHeap 0.
 
 (* Next, some hijinks to prevent unnecessary unfolding of distinct memory cells for the threadq's stack. *)
 
@@ -217,12 +256,20 @@ Definition yieldInvariantCont (pre : vals -> W -> qspec) (rpStashed : bool) (adj
 Local Notation "'PREy' [ vs ] pre" := (yieldInvariantCont (fun vs _ => pre%qspec%Sep))
   (at level 89).
 
+Notation "'badt' name p 'end'" :=
+  {| FName := name;
+    FPrecondition := (fun _ => PropX.Forall p);
+    FBody := Diverge;
+    FVars := nil;
+    FReserved := 0 |}
+  (no associativity, at level 95, name at level 0, p at level 0, only parsing) : SPfuncs_scope.
+
 Definition m := bimport [[ "malloc"!"malloc" @ [mallocS],
     "queue"!"init" @ [Queue.initS], "queue"!"isEmpty" @ [isEmptyS],
     "queue"!"enqueue" @ [enqueueS], "queue"!"dequeue" @ [dequeueS] ]]
   bmodule "threadq" {{
     badt "ADT"
-      tq
+      (fun x => tq (World x) (Pointer x) (Settings x) (Mem x))
     end with bfunction "init"("q", "sp", "r") [initS]
       "q" <-- Call "queue"!"init"()
       [PRE[_, R] mallocHeap 0
@@ -248,28 +295,29 @@ Definition m := bimport [[ "malloc"!"malloc" @ [mallocS],
       "sc" <-* "sc";;
       Note [mergeSusp];;
       Call "queue"!"enqueue"("sc", "pc", "sp")
-      [Al b, Al sc,
-        PRE[V] susps (b %+ (V "pc", V "sp")) sc
-         POST[_] susps (b %+ (V "pc", V "sp")) sc];;
+      [Al w, Al b, Al sc,
+        PRE[V] susps w (b %+ (V "pc", V "sp")) sc
+         POST[_] susps w (b %+ (V "pc", V "sp")) sc];;
       Return 0
     end with bfunction "spawn"("sc", "pc", "ss") [spawnS]
       "ss" <-- Call "malloc"!"malloc"(0, "ss")
-      [Al ss,
-        PRE[V, R] tq (V "sc") * starting (V "sc") (V "pc") (ss - 2) * mallocHeap 0
+      [Al w, Al ss,
+        PRE[V, R] tq w (V "sc") * starting w (V "sc") (V "pc") (ss - 2) * mallocHeap 0
           * R =?> ss * [| (ss >= 2)%nat |]
-        POST[_] tq (V "sc") * mallocHeap 0];;
+        POST[_] tq w (V "sc") * mallocHeap 0];;
 
-      Assert [Al ss, Al vs,
-        PRE[V] tq (V "sc") * starting (V "sc") (V "pc") ss * mallocHeap 0
+      Assert [Al w, Al ss, Al vs,
+        PRE[V] tq w (V "sc") * starting w (V "sc") (V "pc") ss * mallocHeap 0
           * locals ("rp" :: "sc" :: nil) vs ss (V "ss")
-        POST[_] tq (V "sc") * mallocHeap 0];;
+        POST[_] tq w (V "sc") * mallocHeap 0];;
 
       (* Save pointer to threadq data structure in new thread's stack. *)
       "ss" + 4 *<- "sc";;
 
       Assert* [("threadq","ADT")]
-      [PRE[V] tq (V "sc") * susp (V "sc") (V "pc") (V "ss") * mallocHeap 0
-       POST[_] tq (V "sc") * mallocHeap 0];;
+      [Al w,
+        PRE[V] tq w (V "sc") * susp w (V "sc") (V "pc") (V "ss") * mallocHeap 0
+        POST[_] tq w (V "sc") * mallocHeap 0];;
 
       Call "threadq"!"spawnWithStack"("sc", "pc", "ss")
       [PRE[_] Emp
@@ -278,11 +326,11 @@ Definition m := bimport [[ "malloc"!"malloc" @ [mallocS],
     end with bfunctionNoRet "exit"("sc", "q", "r") [exitS]
       "q" <-* "sc";;
       "r" <-- Call "queue"!"isEmpty"("q")
-      [Al q, Al tsp, Al vs,
+      [Al w, Al q, Al tsp, Al vs,
         PREonly[V, R] [| (q %= empty) \is R |]
           * queue q (V "q") * (V "sc" ==*> V "q", tsp)
           * locals ("rp" :: "sc" :: "q" :: "curPc" :: "curSp" :: "newPc" :: "newSp" :: nil) vs 14 tsp          
-          * (V "sc" ^+ $8) =?> 2 * susps q (V "sc") * ginv (V "sc") * mallocHeap 0];;
+          * (V "sc" ^+ $8) =?> 2 * susps w q (V "sc") * ginv w (V "sc") * mallocHeap 0];;
 
       If ("r" = 1) {
         (* No threads left to run.  Let's loop forever! *)
@@ -292,10 +340,10 @@ Definition m := bimport [[ "malloc"!"malloc" @ [mallocS],
 
         "r" <- "sc" + 8;;
         Call "queue"!"dequeue"("q", "r")
-        [Al q, Al tsp, Al pc, Al sp, Al vs,
+        [Al w, Al q, Al tsp, Al pc, Al sp, Al vs,
           PREonly[V] [| (pc, sp) %in q |] * queue (q %- (pc, sp)) (V "q")
-            * susps (q %- (pc, sp)) (V "sc") * susp (V "sc") pc sp
-            * (V "sc" ==*> V "q", tsp, pc, sp) * ginv (V "sc") * mallocHeap 0
+            * susps w (q %- (pc, sp)) (V "sc") * susp w (V "sc") pc sp
+            * (V "sc" ==*> V "q", tsp, pc, sp) * ginv w (V "sc") * mallocHeap 0
             * locals ("rp" :: "sc" :: "q" :: "curPc" :: "curSp" :: "newPc" :: "newSp" :: nil) vs 14 tsp];;
 
         Rp <-* "sc" + 8;;
@@ -306,12 +354,12 @@ Definition m := bimport [[ "malloc"!"malloc" @ [mallocS],
       "q" <-* "sc";;
       (* Using "curPc" as a temporary before getting to its primary use... *)
       "curPc" <-- Call "queue"!"isEmpty"("q")
-      [Al q, Al tsp, Al vs,
+      [Al w, Al q, Al tsp, Al vs,
         PRE[V, R] [| (q %= empty) \is R |]
-          * queue q (V "q") * (V "sc" ==*> V "q", tsp) * (V "sc" ^+ $8) =?> 2 * susps q (V "sc")
-          * ginv (V "sc") * mallocHeap 0
+          * queue q (V "q") * (V "sc" ==*> V "q", tsp) * (V "sc" ^+ $8) =?> 2 * susps w q (V "sc")
+          * ginv w (V "sc") * mallocHeap 0
           * locals ("rp" :: "sc" :: "q" :: "curPc" :: "curSp" :: "newPc" :: "newSp" :: nil) vs 14 tsp * any
-        POST[_] tq (V "sc") * ginv (V "sc") * mallocHeap 0];;
+        POST[_] Ex w', [| evolve w w' |] * tq w' (V "sc") * ginv w' (V "sc") * mallocHeap 0];;
 
       If ("curPc" = 1) {
         (* No other threads to run.  Simply returning to caller acts like a yield. *)
@@ -321,17 +369,18 @@ Definition m := bimport [[ "malloc"!"malloc" @ [mallocS],
         (* Pick a thread to switch to. *)
         "curPc" <- "sc" + 8;;
         Call "queue"!"dequeue"("q", "curPc")
-        [Al q, Al tsp, Al vs, Al pc, Al sp,
+        [Al w, Al q, Al tsp, Al vs, Al pc, Al sp,
           PRE[V] [| (pc, sp) %in q |] * queue (q %- (pc, sp)) (V "q")
-            * susps (q %- (pc, sp)) (V "sc") * susp (V "sc") pc sp
-            * (V "sc" ==*> V "q", tsp, pc, sp) * ginv (V "sc") * mallocHeap 0
+            * susps w (q %- (pc, sp)) (V "sc") * susp w (V "sc") pc sp
+            * (V "sc" ==*> V "q", tsp, pc, sp) * ginv w (V "sc") * mallocHeap 0
             * locals ("rp" :: "sc" :: "q" :: "curPc" :: "curSp" :: "newPc" :: "newSp" :: nil) vs 14 tsp * any
-          POST[_] tq (V "sc") * ginv (V "sc") * mallocHeap 0];;
+          POST[_] Ex w', [| evolve w w' |] * tq w' (V "sc") * ginv w' (V "sc") * mallocHeap 0];;
         "newPc" <-* "sc" + 8;;
         "newSp" <-* "sc" + 12;;
 
-        Assert [PRE[V] susp (V "sc") (V "newPc") (V "newSp") * tq (V "sc") * ginv (V "sc") * mallocHeap 0
-          POST[_] tq (V "sc") * ginv (V "sc") * mallocHeap 0];;
+        Assert [Al w,
+          PRE[V] susp w (V "sc") (V "newPc") (V "newSp") * tq w (V "sc") * ginv w (V "sc") * mallocHeap 0
+          POST[_] Ex w', [| evolve w w' |] * tq w' (V "sc") * ginv w' (V "sc") * mallocHeap 0];;
 
         (* Initialize the temporary stack with data we will need, then switch to using it as our stack. *)
         "curPc" <-* "sc" + 4;;
@@ -345,17 +394,17 @@ Definition m := bimport [[ "malloc"!"malloc" @ [mallocS],
         Sp <- "curPc";;
 
         Assert* [("threadq","ADT")]
-        [PREy[V] Ex sp, Ex b, (V "sc" ==*> V "q", sp) * (V "sc" ^+ $8) =?> 2
-          * queue b (V "q") * susps b (V "sc") * any * ginv (V "sc") * mallocHeap 0
-          * susp (V "sc") (V "newPc") (V "newSp") * susp (V "sc") (V "curPc") (V "curSp")];;
+        [PREy[V] Ex w, Ex sp, Ex b, (V "sc" ==*> V "q", sp) * (V "sc" ^+ $8) =?> 2
+          * queue b (V "q") * susps w b (V "sc") * any * ginv w (V "sc") * mallocHeap 0
+          * susp w (V "sc") (V "newPc") (V "newSp") * susp w (V "sc") (V "curPc") (V "curSp")];;
 
         Note [mergeSusp];;
 
         (* Enqueue current thread; note that variable references below resolve in the temporary stack. *)
         Call "queue"!"enqueue"("q", "curPc", "curSp")
-        [PREy[V] Ex b, Ex p, Ex sp, (V "sc" ==*> p, sp) * (V "sc" ^+ $8) =?> 2
-          * queue b p * susps b (V "sc") * any * ginv (V "sc")
-          * mallocHeap 0 * susp (V "sc") (V "newPc") (V "newSp")];;
+        [PREy[V] Ex w, Ex b, Ex p, Ex sp, (V "sc" ==*> p, sp) * (V "sc" ^+ $8) =?> 2
+          * queue b p * susps w b (V "sc") * any * ginv w (V "sc")
+          * mallocHeap 0 * susp w (V "sc") (V "newPc") (V "newSp")];;
 
         (* Jump to dequeued thread. *)
         "sc" + 4 *<- Sp;;
@@ -368,9 +417,13 @@ Definition m := bimport [[ "malloc"!"malloc" @ [mallocS],
 
 Local Hint Extern 1 (@eq W _ _) => words.
 
-Ltac t := abstract (sep hints; try apply any_easy;
+(*Ltac t := abstract (sep hints; try apply any_easy;
   try (apply himp_star_frame; [ reflexivity | apply susps_del_fwd; assumption ]);
-    eauto).
+    eauto).*)
+
+Ltac t := solve [ sep hints; try apply any_easy;
+  try (apply himp_star_frame; [ reflexivity | apply susps_del_fwd; assumption ]);
+    eauto ].
 
 Lemma wordBound : forall w : W,
   natToW 2 <= w
@@ -387,7 +440,6 @@ Theorem ok : moduleOk m.
   vcgen.
 
   t.
-
   t.
   t.
   t.
@@ -442,27 +494,22 @@ Theorem ok : moduleOk m.
   match goal with
     | [ H : interp _ _ |- _ ] =>
       toFront ltac:(fun P => match P with
-                               | starting _ _ _ => idtac
+                               | starting _ _ _ _ => idtac
                              end) H;
       apply starting_elim in H; post; descend
   end.
   toFront_conc ltac:(fun P => match P with
-                                | susp _ _ _ => idtac
+                                | susp _ _ _ _ => idtac
                               end);
   apply susp_intro; descend.
-  4: instantiate (4 := locals ("rp" :: "sc" :: nil) (upd x2 "sc" (sel x4 "sc")) x1 (sel x4 "ss")); sep_auto.
+  4: instantiate (5 := locals ("rp" :: "sc" :: nil) (upd x3 "sc" (sel x5 "sc")) x2 (sel x5 "ss")); sep_auto.
   eauto.
   eauto.
   eauto.
   eapply Imply_trans; [ | apply H10 ]; clear H10.
+  descend; step auto_ext.
+  eauto.
   step auto_ext.
-  step auto_ext.
-  make_Himp.
-  rewrite H9.
-  repeat (apply Himp_star_frame; try apply Himp_refl).
-  do 3 intro; rewrite sepFormula_eq; unfold predIn, sepFormula_def; simpl.
-  rewrite memoryIn_memoryOut; apply Imply_refl.
-  rewrite sepFormula_eq; apply Himp_refl.
   auto.
   step auto_ext.
   sep_auto.
@@ -488,35 +535,28 @@ Theorem ok : moduleOk m.
   match goal with
     | [ H : interp _ _ |- _ ] =>
       toFront ltac:(fun P => match P with
-                               | susp _ _ _ => idtac
+                               | susp _ _ _ _ => idtac
                              end) H;
       apply susp_elim in H; post
   end.
   descend.
   step auto_ext.
   match goal with
-    | [ H : _ |- _ ] => eapply (Imply_sound (H _)); clear H; eauto
+    | [ H : _ |- _ ] => eapply (Imply_sound (H _ _)); clear H; eauto
   end.
   propxFo.
+  apply evolve_refl.
   unfold labl in H7; rewrite H1 in H7; injection H7; clear H1 H7; intros; subst.
   rewrite H9 in H2; injection H2; clear H2 H9; intros; subst.
-  change (fun st m => subst (globalInv (sel x8 "sc") st m) x10)
-    with (substH (globalInv (sel x8 "sc")) x10).
-  assert (interp specs (![x12 * tq (sel x8 "sc") * ginv (sel x8 "sc") * mallocHeap 0] (stn, st)
-    ---> ![x12 * predIn x10 (sel x8 "sc") * substH (globalInv (sel x8 "sc")) x10 * mallocHeap 0] (stn, st))%PropX).
-  make_Himp; repeat apply Himp_star_frame; try apply Himp_refl.
-  unfold Himp, himp; intros.
-  unfold predIn.
-  change x10 with (fun x => x10 x).
-  rewrite H.
-  rewrite sepFormula_eq; unfold sepFormula_def; simpl.
-  rewrite memoryIn_memoryOut.
-  apply Imply_refl.
-  unfold substH.
-  replace x10 with (predOut tq).
-  apply Himp_refl.
-  symmetry; rewrite sepFormula_eq in H; assumption.
-  apply (Imply_sound H0); clear H0 H.
+  apply (f_equal (fun f => f (stn, st))) in H.
+
+  Require Import Eqdep.
+  injection H; clear H; intros; subst.
+  do 2 apply inj_pair2 in H; subst; simpl.
+  change (fun x y => tq x2 (sel x9 "sc") x y) with (tq x2 (sel x9 "sc")).
+  change (fun st m => subst (globalInv x2 (sel x9 "sc") st m)
+    (fun x : tq_args world => tq (World x) (Pointer x) (Settings x) (Mem x)))
+    with (ginv x2 (sel x9 "sc")).
   step hints; apply any_easy.
 
   t.
@@ -531,8 +571,8 @@ Theorem ok : moduleOk m.
   step hints.
   step hints.
   descend; step hints.
-  instantiate (2 := x7).
-  instantiate (3 := upd x1 "q" x8).
+  instantiate (2 := x8).
+  instantiate (3 := upd x2 "q" x9).
   descend; cancel hints.
   sep hints.
   sep hints.
@@ -541,6 +581,9 @@ Theorem ok : moduleOk m.
   t.
   t.
   t.
+
+  Hint Immediate evolve_refl.
+
   t.
   t.
 
@@ -550,8 +593,8 @@ Theorem ok : moduleOk m.
   eauto.
   step hints.
   descend; step hints.
-  instantiate (2 := x2).
-  instantiate (3 := upd (upd x5 "curPc" (Regs x0 Rv)) "curPc" (sel x5 "sc" ^+ $8)).
+  instantiate (2 := x3).
+  instantiate (3 := upd (upd x6 "curPc" (Regs x0 Rv)) "curPc" (sel x6 "sc" ^+ $8)).
   descend; cancel hints.
   step hints.
   apply himp_star_frame; [ reflexivity | apply susps_del_fwd; assumption ].
@@ -565,44 +608,37 @@ Theorem ok : moduleOk m.
 
   post; evaluate hints.
   descend.
-  instantiate (1 := upd (upd (upd (upd (upd (upd x6 "sc" (sel x2 "sc")) "q" x8) "curPc"
-    (sel x2 "rp")) "curSp" (Regs x0 Sp)) "newPc" (sel x2 "newPc")) "newSp" (sel x2 "newSp")); descend.
+  instantiate (1 := upd (upd (upd (upd (upd (upd x7 "sc" (sel x3 "sc")) "q" x9) "curPc"
+    (sel x3 "rp")) "curSp" (Regs x0 Sp)) "newPc" (sel x3 "newPc")) "newSp" (sel x3 "newSp")); descend.
   toFront_conc ltac:(fun P => match P with
-                                | susp _ (sel _ "rp") _ => idtac
+                                | susp _ _ (sel _ "rp") _ => idtac
                               end).
   apply susp_intro; descend; eauto.
   match goal with
     | [ _ : context[locals ?ns ?v ?a (Regs ?st Sp)] |- interp specs (![?P * _] _) ] =>
-      equate P (locals ns v a (Regs st Sp) * (fun x y => x1 (x, y)))%Sep
+      equate P (locals ns v a (Regs st Sp) * (fun x y => x2 (x, y)))%Sep
   end.
   step hints.
   step auto_ext.
   step auto_ext.
-  match goal with
-    | [ |- interp _ (![?P * ?Q * ?R * ?S * ?T] _ ---> _)%PropX ] =>
-      let H := fresh in assert (H : P * Q * R * S * T ===> P * Q * tq (sel x2 "sc") * ginv (sel x2 "sc") * T); [
-        | eapply Imply_trans; [ rewrite sepFormula_eq in *; apply H | ] ]
-  end.
-  repeat apply Himp_star_frame; try apply Himp_refl.
-  do 3 intro; rewrite sepFormula_eq; unfold sepFormula_def, predIn; simpl.
-  rewrite memoryIn_memoryOut; apply Imply_refl.
-  rewrite sepFormula_eq; apply Himp_refl.
-  match goal with
-    | [ |- interp _ (?P ?x ?y ---> _) ] => change (P x y) with (sepFormula_def P (s, s0))
-  end; rewrite <- sepFormula_eq.
-  instantiate (1 := upd (upd x2 "curPc" x7) "q" x8); clear.
+  change (fun (x11 : ST.settings) (y : smem) => tq w' (sel x3 "sc") x11 y)
+    with (tq w' (sel x3 "sc")).
+  change (fun (st : ST.settings) (m0 : smem) =>
+    subst (globalInv w' (sel x3 "sc") st m0)
+      (fun x11 : tq_args world =>
+        tq (World x11) (Pointer x11) (Settings x11) (Mem x11))) with (ginv w' (sel x3 "sc")).
   step auto_ext.
 
   t.
   t.
 
   post; evaluate hints; descend.
-  instantiate (3 := x2).
+  instantiate (3 := x3).
   step hints.
   step hints.
   step hints.
   unfold yieldInvariantCont; descend; step hints.
-  instantiate (6 := x2 %+ (sel x0 "curPc", sel x0 "curSp")).
+  instantiate (8 := x3 %+ (sel x0 "curPc", sel x0 "curSp")).
   descend; step hints.
 
   t.
@@ -612,35 +648,26 @@ Theorem ok : moduleOk m.
   match goal with
     | [ H : interp _ _ |- _ ] =>
       toFront ltac:(fun P => match P with
-                               | susp _ _ _ => idtac
+                               | susp _ _ _ _ => idtac
                              end) H;
       apply susp_elim in H; post
   end.
   descend.
   step auto_ext.
   match goal with
-    | [ H : _ |- _ ] => eapply (Imply_sound (H _)); eauto
+    | [ H : _ |- _ ] => eapply (Imply_sound (H _ _)); eauto
   end.
   unfold labl in H7; rewrite H1 in H7; injection H7; clear H1 H7; intros; subst.
   rewrite H8 in H2; injection H2; clear H2 H8; intros; subst.
-  change (fun (st0 : ST.settings) (m0 : smem) => subst (globalInv (sel x2 "sc") st0 m0) x8)
-    with (substH (globalInv (sel x2 "sc")) x8).
-  assert (interp specs (![x10 * tq (sel x2 "sc") * ginv (sel x2 "sc") * mallocHeap 0] (stn, st)
-    ---> ![x10 * predIn x8 (sel x2 "sc") * substH (globalInv (sel x2 "sc")) x8 * mallocHeap 0] (stn, st))%PropX).
-  make_Himp; repeat apply Himp_star_frame; try apply Himp_refl.
-  unfold Himp, himp; intros.
-  unfold predIn.
-  change x8 with (fun x => x8 x).
-  rewrite H1.
-  rewrite sepFormula_eq; unfold sepFormula_def; simpl.
-  rewrite memoryIn_memoryOut.
-  apply Imply_refl.
-  unfold ginv.
-  replace (predOut tq) with x8.
-  apply Himp_refl.
-  rewrite sepFormula_eq in *; assumption.
+  apply (f_equal (fun f => f (stn, st))) in H1.
+  injection H1; clear H1; intros; subst.
+  do 2 apply inj_pair2 in H1; subst; simpl.
+  instantiate (1 := x3).
+  change (fun x y => tq x3 (sel x2 "sc") x y) with (tq x3 (sel x2 "sc")).
+  change (fun st m => subst (globalInv x3 (sel x2 "sc") st m)
+    (fun x : tq_args world => tq (World x) (Pointer x) (Settings x) (Mem x)))
+    with (ginv x3 (sel x2 "sc")).
   propxFo.
-  apply (Imply_sound H2); clear H2 H1.
   step hints.
 Qed.
 
